\input{stdinclude.tex}
\begin{document}

\mainHeaderDiff{13}{Inverse Functions}
A function is one-to-one (or injective) if $ f(x) = f(y) $ implies that $ x = y $ (i.e. two different inputs can never
give the same output/the function passes the horizontal-line test).

\begin{defn}
  Let $ f $ be a function that is one-to-one. Then the \textbf{inverse} of $ f $ is the (unique) function $ f^{-1} $ such that
  \begin{displaymath}
    f(x) = y \iff f^{-1}(y) = x.
  \end{displaymath}
  In other words, $ f(f^{-1}(y)) = y $ and $ f^{-1}(f(x)) = x $.
\end{defn}

\begin{ex}
  Here are some functions with their inverses:
  \begin{center}
  \def\arraystretch{1.5}
  \begin{tabularx}{0.9\linewidth}{|c|c|X|}\hline
    \textbf{Function} & \textbf{Inverse} & \textbf{Notes}\\\hline
    $ e^x $ & $ \ln x $ & Note that $ \ln x $ is defined only when $ x > 0 $ since $ e^x > 0 $ for all real $ x $.\\
    $ \sin x $ & $ \sin^{-1} x $ & Note that $ \sin^{-1} x $ is only defined when $ -\pi < x \leq \pi $ since otherwise $ \sin x $ is not one-to-one.\\
    $ \cos x $ & $ \cos^{-1} x $ & Note that $ \cos^{-1} x $ is only defined when $ -\pi < x \leq \pi $ since otherwise $ \cos x $ is not one-to-one.\\
    $ \tan x $ & $ \tan^{-1} x $ & Note that $ \tan^{-1} x $ is defined for all $ x $ (why?), and so $ \tan^{-1} x \neq \frac{\sin^{-1} x}{\cos^{-1} x} $.\\
    $ x^2 $ & $ \sqrt{x} $ & When $ x $ is positive.\\\hline
  \end{tabularx}
  \end{center}
\end{ex}
The graph of the inverse of a function is the reflection of the graph of the original function around the line $ x = y $ (essentially, we swap
the $ x $ and $ y $ axes).

In order to illustrate the general process of finding the derivatives of inverse functions, let us now find the derivative of $ y = \sin^{-1} x $.
\begin{align*}
  y &= \sin^{-1} x\\
  \sin y &= x\\
  \dod{y}{x} \cos y &= 1\\
  \dod{y}{x} &= \frac{1}{\cos y} = \frac{1}{\cos \sin^{-1} x} = \frac{1}{\sqrt{1 - x^2}}.
\end{align*}
The identity $ \cos\sin^{-1} x = \sqrt{1 - x^2} $ comes from the following triangle:
\begin{center}
  \includegraphics[width=0.2\textwidth]{antitriangle}
\end{center}

It is possible to write down an expression relating the derivative of $ f^{-1} $ to the derivative of $ f $. However, in the immortal words of
Michael~Artin, ``even mathematicians occasionally feel that isn't worthwhile making a precise formulation --- that it is easier to consider each
case as it comes along. This is one of those occasions.''\footnote{~Artin, \textit{Algebra} (1st ed), p.457.} (The general theorem is given in
the exercises below for you to prove.)

\clearpage
By the same kind of calculation, we obtain the following table which gives the derivatives of inverses of the three primary trigonometric
functions and their reciprocals.
\begin{center}
  \def\arraystretch{1.8}
  \begin{tabular}{|c|c|c|c|}\hline
    \textbf{Function} & \textbf{Derivative} &
    \textbf{Function} & \textbf{Derivative}\\\hline
    $ \sin^{-1} x $ & $ \dfrac{1}{\sqrt{1 - x^2}} $ &
    $ \csc^{-1} x $ & $ -\dfrac{1}{x\sqrt{x^2 - 1}} $ \\\hline
    $ \cos^{-1} x $ & $ -\dfrac{1}{\sqrt{1 - x^2}} $ &
    $ \sec^{-1} x $ & $ \dfrac{1}{x\sqrt{x^2 - 1}} $\\\hline
    $ \tan^{-1} x $ & $ \dfrac{1}{1+x^2} $ &
    $ \cot^{-1} x $ & $ -\dfrac{1}{x^2 + 1}$\\\hline
  \end{tabular}
\end{center}

\subsection*{Questions}
\begin{questions}
  \questioM Prove or disprove the following statements:
    \begin{parts}
      \part The function $ f : x \mapsto x^2 + x + 1 $ is one-to-one (where $ x $ is real).
      \part The function $ g : x \mapsto 2^x $ is one-to-one (where $ x $ is a positive real).
    \end{parts}
  \questioM Determine whether the following functions have inverses on the given interval:
    \begin{parts}
      \part $ x \mapsto x^3 $ (on $ \mathbb{R} $)
      \part $ y \mapsto y^4 $ (on $ \mathbb{R} $)
      \part $ y \mapsto y^4 $ (for $ y \geq 0 $)
      \part $ y \mapsto y^4 $ (for $ y > 0 $)
      \part $ \theta \mapsto \cos^{-1} \theta $ (on $ \mathbb{R} $)
      \part $ \theta \mapsto \cos^{-1} \theta $ (for $ -1 \leq \theta \leq 1 $)
    \end{parts}
  \questioA True or false:
    \begin{parts}
      \part $ \cos^{-1} x = \frac{1}{\cos x} $
      \part If $ x > 0 $ then $ (\ln x)^6 = 6\ln x $
      \part $ \tan^{-1} (-1) = \frac{3\pi}{4} $ (think about which arm of $ \tan x $ we're talking about)
      \part The inverse of $ f(x) = e^{3x} $ is $ f^{-1}(x) = \frac{1}{3} \ln x $.
    \end{parts}
  \questioA Find the derivative of $ f(x) = \ln(e^x) $ in two different ways.
  \questioA Find $ y' $ if:
    \begin{parts}
      \part $ y = \sin^{-1} 2x $
      \part $ x = \sin^2 y $
      \part $ y = x + \tan^{-1} y $
      \part $ y = \ln \sin x - \frac{1}{2} \sin^2 x $
      \part $ y = 24\arctan x + \arcsin \sqrt{x} $
      \part $ y = \sqrt{\sec^{-1} 2x} $
    \end{parts}
  \clearpage
  \questioE Find the local extrema, areas of concavity, and inflection points of the following functions; hence sketch their graphs.
    \begin{parts}
      \part $ y = e^x \sin x $ for $ -\pi < x < \pi $
      \part $ y = x + \ln(x^2 + 1) $
      \part $ y = \sin^{-1} (1/x) $
    \end{parts}
  \questioE Justify intuitively, without invoking the happy coincidence that our notation for derivatives looks like a fraction, the
            statement that $ \od{y}{x} = \left(\od{x}{y}\right)^{-1} $.
  \questioE If $ f'(x) = \tan^{-1} x $, find $ (f^{-1})'(x) $.
  \questioE Suppose $ f $ is a function, and $ f^{-1} $ is the inverse of $ f $. Prove that $ (f^{-1})'(y) = \frac{1}{f'(f^{-1}(y))} $.
  \questioS Prove the formulae for the derivatives of $ \cos^{-1} $ and $ \tan^{-1} $, using a similar method to that for $ \sin^{-1} x $.
  \questioS Scholarship 2012: Consider the equation $ x^n = \tan(ny) $, where $ n $ is a constant. Find an expression
            for $ \od{y}{x} $ in terms of $ x $.
\end{questions}
\end{document}
